cedar-lean/DiffTest/Parser.lean
@@ -412,11 +412,11 @@ def descendantsToAncestors [LT α] [BEq α] [DecidableLT α] (descendants : Map 
   Map.make (List.map
     (λ (k,_) => (k, findInMapValues descendants k)) descendants.toList)
 
-structure JsonEntityTypeStoreEntry where
+structure JsonEntitySchemaEntry where
   descendants : Cedar.Data.Set EntityType
   attrs : RecordType
 
-abbrev JsonEntityTypeStore := Map EntityType JsonEntityTypeStoreEntry
+abbrev JsonEntitySchema := Map EntityType JsonEntitySchemaEntry
 
 structure JsonSchemaActionEntry where
   appliesToPrincipal : Set EntityType
@@ -426,7 +426,7 @@ structure JsonSchemaActionEntry where
 
 abbrev JsonSchemaActionStore := Map EntityUID JsonSchemaActionEntry
 
-def invertJsonEntityTypeStore (ets : JsonEntityTypeStore) : EntityTypeStore :=
+def invertJsonEntitySchema (ets : JsonEntitySchema) : EntitySchema :=
   let ets := ets.toList
   let descendantMap := Map.make (List.map (λ (k,v) => (k,v.descendants)) ets)
   let ancestorMap := descendantsToAncestors descendantMap
@@ -491,7 +491,7 @@ partial def jsonToCedarType (json : Lean.Json) : ParseResult CedarType := do
       .ok (.ext name)
     | tag => .error s!"jsonToCedarType: unknown tag {tag}"
 
-partial def jsonToEntityTypeEntry (json : Lean.Json) : ParseResult JsonEntityTypeStoreEntry := do
+partial def jsonToEntityTypeEntry (json : Lean.Json) : ParseResult JsonEntitySchemaEntry := do
   let descendants_json ← getJsonField json "descendants" >>= jsonToArray
   let descendants ← List.mapM jsonToName descendants_json.toList
   let attrs ← getJsonField json "attributes" >>= (getJsonField · "attrs") >>= jsonToRecordType
@@ -525,7 +525,7 @@ partial def jsonToSchema (json : Lean.Json) : ParseResult Schema := do
   let actionsKVs ← getJsonField json "actionIds" >>= jsonArrayToKVList
   let actions ← mapMKeysAndValues actionsKVs jsonToEuid jsonToSchemaActionEntry
   .ok {
-    ets := invertJsonEntityTypeStore (Map.make entityTypes),
+    ets := invertJsonEntitySchema (Map.make entityTypes),
     acts := invertJsonSchemaActionStore (Map.make actions)
   }
 
